Fix ClassTable to lookup frorefinements from last to first

src/FFJ/ClassTable.v
@@ -25,23 +25,20 @@ Tactic Notation "subtype_cases" tactic(first) ident(c) :=
   [ Case_aux c "S_Refl" | Case_aux c "S_Trans" 
   | Case_aux c "S_Decl"].
 
-Inductive succ: ClassName + RefinementName -> RefinementName -> Prop :=
-  | Class_succ : forall C CR,
-    head (refinements_of C) = Some CR ->
-    succ (inl C) (class_name CR @ ref CR)
-  | Refine_succ : forall C Rs feat n CR,
+Inductive pred: RefinementName -> RefinementName -> Prop :=
+  | P_Refine : forall C Rs feat n CR,
     refinements_of C = Rs ->
-    find_where feat (refs Rs) = Some n ->
-    nth_error Rs (S n) = Some CR ->
-    succ (inr (C @ feat)) (class_name CR @ ref CR).
+    find_where feat (refs Rs) = Some (S n) ->
+    nth_error Rs n = Some CR ->
+    pred (class_name CR @ ref CR) (C @ feat).
 
-(* pred is just the inverse of succ *)
-Inductive pred (R: RefinementName) (Cl: ClassName + RefinementName): Prop :=
+(* pred is just the inverse of succ
+Inductive succ (Cl: ClassName + RefinementName) (R: RefinementName): Prop :=
   | C_pred: 
-    succ Cl R ->
-    pred R Cl.
-
-(* Refinement is the transitive closure of succ *)
+    pred R Cl ->
+    succ Cl R.
+*)
+(* Refinement is the transitive closure of succ 
 Reserved Notation "C <<: D" (at level 40).
 Inductive Refinement: ClassName + RefinementName -> RefinementName -> Prop :=
   | R_Trans: forall C C' C'',
@@ -52,6 +49,7 @@ Inductive Refinement: ClassName + RefinementName -> RefinementName -> Prop :=
     succ C C' ->
     C <<: C'
 where "C <<: C'" := (Refinement C C').
+*)
 
 Definition last_refinement (C: ClassName): option RefinementName :=
   match last_error (refinements_of C) with
@@ -59,28 +57,28 @@ Definition last_refinement (C: ClassName): option RefinementName :=
   | NOne => None
   end.
 
-Definition no_suc (R: ClassName + RefinementName) : Prop := forall S, ~succ R S.
-
+Definition first_refinement (R: RefinementName) : Prop := forall S, ~pred R S.
+(*
 Lemma last_refinement_correct: forall C R,
   last_refinement C = Some R <-> no_suc (inr (class_name R @ ref R)).
 Proof. (* Need to impose that there are no duplicated features *)
 Admitted.
-
+*)
 
 Inductive fields_refinement : RefinementName -> [FieldDecl] -> Prop :=
   | F_Refine: forall R S fs fpred noDupfDecls K mDecls noDupmDecls mRefines noDupmRefines,
-    pred R (inr S) ->
+    pred R S ->
     find_refinement R (CRefine R fs noDupfDecls K mDecls noDupmDecls mRefines noDupmRefines) ->
     fields_refinement S fpred ->
     NoDup (refs (fpred ++ fs)) ->
     fields_refinement R (fpred ++ fs)
-  | F_First: forall C R fs noDupfDecls K mDecls noDupmDecls mRefines noDupmRefines,
-    pred R (inl C) ->
+  | F_First: forall R fs noDupfDecls K mDecls noDupmDecls mRefines noDupmRefines,
+    first_refinement R ->
     find_refinement R (CRefine R fs noDupfDecls K mDecls noDupmDecls mRefines noDupmRefines) ->
     fields_refinement R fs.
 
-Hint Constructors succ pred Refinement.
-Hint Unfold last.
+Hint Constructors pred.
+Hint Unfold first_refinement.
 
 Inductive fields : ClassName -> [FieldDecl] -> Prop :=
   | F_Obj : fields Object nil
@@ -101,6 +99,7 @@ Tactic Notation "fields_cases" tactic(first) ident(c) :=
   first;
   [ Case_aux c "F_Obj" | Case_aux c "F_Decl"| Case_aux c "F_Decl_NoRefine"].
 
+(*
 Inductive rfields : ClassName + RefinementName -> [FieldDecl] -> Prop :=
   | RF_Decl : forall C D fs noDupfs K mds noDupMds fs',
      find C CT = Some (CDecl C D fs noDupfs K mds noDupMds) ->
@@ -113,6 +112,7 @@ Inductive rfields : ClassName + RefinementName -> [FieldDecl] -> Prop :=
      rfields P fs' ->
      NoDup (refs (fs' ++ fs)) ->
      rfields (inr R) (fs'++fs).
+*)
 
 Reserved Notation "'mtype_r(' m ',' R ')' '=' c '~>' c0" (at level 40, c at next level).
 Inductive mtype_refinement (m: id) (R: RefinementName) (Bs: [ClassName]) (B: ClassName): Prop :=
@@ -124,7 +124,7 @@ Inductive mtype_refinement (m: id) (R: RefinementName) (Bs: [ClassName]) (B: Cla
   | mtyr_succ: forall S fs noDupfDecls K mDecls noDupmDecls mRefines noDupmRefines,
               find_refinement R (CRefine R fs noDupfDecls K mDecls noDupmDecls mRefines noDupmRefines) ->
               find m mDecls = None ->
-              succ (inr R) S ->
+              pred R S ->
               mtype_r(m, S) = Bs ~> B ->
               mtype_r(m, R) = Bs ~> B
   where "'mtype_r(' m ',' R ')' '=' cs '~>' c0"
@@ -140,13 +140,13 @@ Inductive m_type (m: id) (C: ClassName) (Bs: [ClassName]) (B: ClassName) : Prop:
   | mty_no_override: forall D Fs K Ms noDupfs noDupMds,
               find C CT = Some (CDecl C D Fs noDupfs K Ms noDupMds) ->
               find m Ms = None ->
-              (forall S Bs' B', succ (inl C) S -> ~mtype_r(m, S) = Bs' ~> B') ->
+              (forall S Bs' B', last_refinement C = Some S -> ~mtype_r(m, S) = Bs' ~> B') ->
               mtype(m, D) = Bs ~> B ->
               mtype(m, C) = Bs ~> B
   | mty_refinement: forall D S Fs K Ms noDupfs noDupMds,
               find C CT = Some (CDecl C D Fs noDupfs K Ms noDupMds) ->
               find m Ms = None ->
-              succ (inl C) S ->
+              last_refinement C = Some S ->
               mtype_r(m, S) = Bs ~> B ->
               mtype(m, C) = Bs ~> B
   where "'mtype(' m ',' D ')' '=' cs '~>' c0"
@@ -172,7 +172,7 @@ Inductive mbody_refinement (m: id) (R: RefinementName) (xs: [id]) (e: Exp): Prop
   | mbodyr_succ: forall S fs noDupfDecls K mDecls noDupmDecls mRefines noDupmRefines,
               find_refinement R (CRefine R fs noDupfDecls K mDecls noDupmDecls mRefines noDupmRefines) ->
               find m mDecls = None ->
-              pred R (inr S) ->
+              pred R S ->
               mbody_r(m, S) = xs o e ->
               mbody_r(m, R) = xs o e
   where "'mbody_r(' m ',' R ')' '=' xs 'o' e"
@@ -184,17 +184,18 @@ Inductive m_body (m: id) (C: ClassName) (xs: [ClassName]) (e: Exp) : Prop:=
               find C CT = Some (CDecl C D Fs noDupfs K Ms noDupMds) ->
               find m Ms = Some (MDecl C0 m fargs noDupfargs e) ->
               refs fargs = xs ->
-              (forall S xs' e', succ (inl C) S -> ~ mbody_r(m, S) = xs' o e') ->
+              (forall S xs' e', last_refinement C = Some S ->
+                                ~ mbody_r(m, S) = xs' o e') ->
               mbody(m, C) = xs o e
   | mbody_no_override: forall D Fs K Ms noDupfs noDupMds,
               find C CT = Some (CDecl C D Fs noDupfs K Ms noDupMds) ->
               find m Ms = None ->
-              (forall S xs' e', succ (inl C) S -> ~ mbody_r(m, S) = xs' o e') ->
+              (forall S xs' e', last_refinement C = Some S ->
+                                ~ mbody_r(m, S) = xs' o e') ->
               mbody(m, D) = xs o e ->
               mbody(m, C) = xs o e
   | mbody_last : forall S,
-              (inl C) <<: S -> 
-              no_suc (inr S) ->
+              last_refinement C = Some S -> 
               mbody_r(m, S) = xs o e ->
               mbody(m, C) = xs o e
   where "'mbody(' m ',' D ')' '=' xs 'o' e" := (m_body m D xs e).
@@ -213,11 +214,11 @@ Inductive override (m: id) (D: ClassName) (Cs: [ClassName]) (C0: ClassName): Pro
 
 Inductive introduce (m: id) (R: RefinementName): Prop :=
   | I_Refinement : forall S,
-    pred R (inr S) ->
+    pred R S ->
     (forall Ds D0, ~ mtype_r(m, S) = Ds ~> D0) ->
     introduce m R
-  | I_Class : forall C,
-    pred R (inl C) ->
+  | I_Class : forall C feat,
+    first_refinement R -> R = C @ feat ->
     (forall Ds D0, ~ mtype(m, C) = Ds ~> D0) ->
     introduce m R.
 
@@ -233,25 +234,25 @@ Proof.
   intros. apply find_ref_inv in H. auto.
 Qed.
 
-Lemma succ_same_cname: forall Cl R,
-  succ Cl R ->
+Lemma pred_same_cname: forall Cl R,
+  pred Cl R ->
   class_name Cl = class_name R.
 Proof.
-  induction 1; crush.
-  destruct refinements_same_name with C; crush.
-  destruct refinements_same_name with C; eauto. inversion H1.
-  subst. apply nth_error_In in H1.
-  eapply Forall_forall in f; eauto. rewrite f. eauto.
+  induction 1; crush. destruct CR. destruct r.
+  lets ?H: refinements_same_name C.
+  apply nth_error_In in H1. rewrite Forall_forall in H. eapply H in H1.
+  eauto.
 Qed.
 
+(*
 Lemma refinement_same_cname : forall R Cl,
   Cl <<: R ->
   class_name R = class_name Cl.
 Proof.
-  destruct 1; 
+  destruct 1.  apply pred_same_cname in H.
   repeat match goal with
-  | H: succ ?C ?R |- _ => apply succ_same_cname in H
+  | H: pred ?R ?C |- _ => apply pred_same_cname in H
   end; crush.
 Qed. 
-
-Hint Resolve find_class_same_ref succ_same_cname refinement_same_cname.
+*)
+Hint Resolve find_class_same_ref pred_same_cname.
